ver2/misc.v
@@ -1,6 +1,7 @@
 Require Import List.
 Import ListNotations.
 
+Require Import Arith.
 Require Import Nat.
 Require Import Bool.
 
@@ -41,91 +42,6 @@ Definition fold_right_option {A B : Type} (f: A -> option B)  :=
                   end
     end.
 
-  
-Fixpoint app_f_succ_all {A B: Type} (f: A -> option B) (l: list A) : bool :=
-  match l with
-  | [] => true
-  | x::l' =>
-      match (f x) with
-      | None => false
-      | Some _ => app_f_succ_all f l'
-      end
-  end.
- 
-Lemma app_f_succ_all_tl:
-  forall (A B: Type) (f: A->option B) (l: list A) (a: A),
-    app_f_succ_all f (a::l) = true ->  app_f_succ_all f l = true.
-Proof.
-  intros.
-  unfold app_f_succ_all in H.
-  destruct (f a) in H.
-  + apply H.
-  + discriminate H.
-Qed.
-
-Lemma fold_right_option_succ:
-  forall (A B: Type) (f: A->option B) (l: list A),
-    app_f_succ_all f l = true ->  exists lr, fold_right_option f l = Some lr.
-
-Proof.
-  intros A B f l.
-  induction l as [|a l' IHl'].
-  - intros. exists []. reflexivity.
-  - simpl. destruct (f a) eqn:fa.
-    + intro. apply IHl' in H. destruct H. exists (b::x). rewrite H. reflexivity.
-    + intro. discriminate.
-Qed.      
-
-
-Lemma fold_right_option_len:
-  forall (A B: Type) (f: A->option B) (l1: list A) (l2: list B),
-    fold_right_option f l1 = Some l2 ->
-    length l1 = length l2.
-Proof.
-  induction l1 as [|a l1' IHl1'].
-  - intros. simpl in H. injection H. intros. rewrite <- H0. reflexivity.
-  - intros.
-    unfold fold_right_option in H.
-    destruct (f a).
-    + destruct ((fix fold_right_option_fix (l : list A) : option (list B) :=
-           match l with
-           | [] => Some []
-           | elem :: rs =>
-               match f elem with
-               | Some elem_val =>
-                   match fold_right_option_fix rs with
-                   | Some rs_val => Some (elem_val :: rs_val)
-                   | None => None
-                   end
-               | None => None
-               end
-           end) l1') eqn:E0.
-      ++ apply IHl1' in E0.
-         injection H. intros.
-         rewrite <- H0.
-         simpl. rewrite E0. reflexivity.
-      ++ discriminate.
-    + discriminate.
-Qed.
-
-
-(*
-Alternative implementation of fold_right_option, using List.fold_right
-*)
-Definition fold_right_option_2 {A B : Type} (f: A -> option B) (l: list A) : option (list B) :=
-  let ff := fun b a =>
-             match a with
-             | None => None
-             | Some xs =>
-                 match (f b) with
-                 | None => None
-                 | Some v => Some (v::xs)
-                 end
-             end
-  in
-  fold_right ff (Some []) l.
-
-
 
 (******* stack manipulation operators ********)
 
@@ -159,6 +75,119 @@ Definition swap {T: Type} (k : nat) (stk: list T) : option (list T) :=
        | (Some v, h::t) => Some ([v] ++ ((firstn (k-1) t)) ++ [h] ++ (skipn (k+1) stk))
        | _ => None
        end.
+
+
+(** Facts about functions defined in this module **)
+
+
+(* Just a relation between fold_right_option and its inner function
+fold_right_option_fix. Trivial, but useful for induction and for
+readability *)
+Lemma fold_right_option_ho:
+  forall A B f l,
+  fold_right_option f l =
+    (fix fold_right_option_fix (l: list A) : option (list B) :=
+    match l with 
+    | nil => Some []
+    | elem::rs => let elem_oval := f elem in
+                  let rs_oval := fold_right_option_fix rs in
+                  match (elem_oval, rs_oval) with 
+                  | (Some elem_val, Some rs_val) => Some (elem_val::rs_val)
+                  | _ => None
+                  end
+    end) l.
+Proof.
+  reflexivity.
+Qed.
+
+  
+(* When fold_right_option succeeds, the length of the result list is
+  as the length of the input list *)
+Lemma fold_right_option_len:
+  forall (A B: Type) (f: A->option B) (l1: list A) (l2: list B),
+    fold_right_option f l1 = Some l2 ->
+    length l1 = length l2.
+Proof.
+  intros A B f.
+  induction l1 as [|a l1' IHl1'].
+  - intros l2 H_fold_r_nil.
+    simpl in  H_fold_r_nil.
+    injection  H_fold_r_nil as H_l2.
+    rewrite <- H_l2.
+    reflexivity.
+  - intros l2 H_fold_r_cons.
+    unfold fold_right_option in H_fold_r_cons.
+    destruct (f a) eqn:E_fa.
+    + rewrite <- fold_right_option_ho in H_fold_r_cons.
+      destruct (fold_right_option f l1') eqn:E_fold_r_l1' in H_fold_r_cons.
+      ++ apply IHl1' in E_fold_r_l1'.
+         injection H_fold_r_cons as H_fold_r_cons. 
+         rewrite <- H_fold_r_cons.
+         simpl.
+         rewrite E_fold_r_l1'.
+         reflexivity.
+      ++ discriminate H_fold_r_cons.
+    + discriminate H_fold_r_cons.
+Qed.
+
+(* when fold_right_option succeeds on v::l1 and results in v::l2, and
+l2 is the result of applying fold_right_option on l1.
+*)
+
+Lemma fold_right_option_hd:
+  forall (A B: Type) (f: A->option B) (l1: list A) (l2: list B) (v : A) (e: B),
+    fold_right_option f (v::l1) = Some (e::l2) ->
+    f v = Some e /\ fold_right_option f l1 = Some l2.
+Proof.
+  intros A B f l1 l2 v e H_fold_r.
+  unfold fold_right_option in H_fold_r.
+  rewrite <- fold_right_option_ho in H_fold_r.
+  destruct (f v) eqn:E_fv.
+  + destruct (fold_right_option f l1) eqn:E_fold_r.
+    ++ injection H_fold_r as H_b H_l2.
+       rewrite H_b. rewrite H_l2.
+       split; reflexivity.
+    ++ discriminate.
+  + discriminate.
+Qed.
+
+  
+(* When fold_right_option succeeds, the i-th element of the output is
+the result of applying f to the i-th element in the input.  *)
+Lemma fold_right_option_nth:
+  forall (A B: Type) (f: A->option B) (l1: list A) (l2: list B),
+    fold_right_option f l1 = Some l2 ->
+    forall k,
+      k < length l1 ->
+      exists v,
+        nth_error l1 k = Some v /\
+          nth_error l2 k = f v.
+Proof.
+  intros A B f.
+  induction l1 as [|e l1' IHl1'].
+  - intros l2 H_fold_r_nil k H_k_lt_len.
+    rewrite <- Nat.ltb_lt in H_k_lt_len.
+    simpl in H_k_lt_len.
+    destruct k; discriminate.
+  - intros l2 H_fold_r_cons k H_k_lt_len.
+    destruct l2 eqn:E_l2.
+    + unfold fold_right_option in H_fold_r_cons.
+      rewrite <- fold_right_option_ho in H_fold_r_cons.
+      destruct (f e) eqn:E_fa.
+      ++ destruct (fold_right_option f l1') eqn:E_fold_r_l1' in H_fold_r_cons; discriminate.
+      ++ discriminate.
+    + apply fold_right_option_hd in H_fold_r_cons.
+      destruct H_fold_r_cons as [H_hd H_tl].
+      destruct k eqn:E_k.
+      ++ simpl.
+         rewrite <- H_hd.
+         exists e.
+         split; reflexivity.
+      ++ simpl.
+         simpl in H_k_lt_len. apply lt_S_n in H_k_lt_len.
+         pose proof (IHl1' l H_tl n   H_k_lt_len) as IH.
+         apply IH.
+Qed.
 
 
 End Misc.
